mc_reify/reify.v
@@ -184,11 +184,11 @@ Reify Pattern patterns_vst += (!!tc_temp_id_b_norho @ ?0 @ ?1 ) =>
   (fun (a : id positive) (b : id Ctypes.type) =>
      (@Inj typ func (inr (Smx (ftc_temp_id_b_norho a b ))))).
 
-Reify Pattern patterns_vst += (!!msubst_eval_expr_norho @ ?0 @ ?1 @ ?2) =>
+Reify Pattern patterns_vst += (!!msubst_eval_expr @ ?0 @ ?1 @ ?2) =>
 (fun (a b : function reify_vst) (e : id Clight.expr) =>
 rmsubst_eval_expr a b e).
 (*(@Inj typ func (inr (Smx fmsubst_eval_expr_norho))).*)
-Reify Pattern patterns_vst += (!!msubst_eval_lvalue_norho) => (@Inj typ func (inr (Smx fmsubst_eval_lvalue_norho))).
+Reify Pattern patterns_vst += (!!msubst_eval_lvalue) => (@Inj typ func (inr (Smx fmsubst_eval_lvalue_norho))).
 
 
 
