mc_reify/set_load_store.v
@@ -1,0 +1,31 @@
+Require Import floyd.proofauto. 
+Require Import mc_reify.bool_funcs.
+Local Open Scope logic.
+
+Lemma semax_PTree_set:
+  forall {Espec: OracleKind},
+    forall Delta id P T1 T2 R (e2: Clight.expr) t v,
+      typeof_temp Delta id = Some t ->
+      is_neutral_cast (implicit_deref (typeof e2)) t = true ->
+      msubst_eval_expr T1 T2 e2 = Some v ->
+      (local (tc_environ Delta)) && (assertD P (localD T1 T2) R) |--
+        local (tc_expr Delta e2) ->
+      semax Delta (|> (assertD P (localD T1 T2) R))
+        (Sset id e2)
+          (normal_ret_assert
+            (assertD P (localD (PTree.set id v T1) T2) R)).
+Proof.
+  intros.
+  unfold assertD, localD in *.
+  rewrite insert_local in H2.
+  eapply semax_post'.
+  Focus 2. {
+    eapply semax_SC_set; eauto.
+    instantiate (1 := v).
+    rewrite <- insert_local.
+    apply andp_left2.
+    apply msubst_eval_expr_eq, H1.
+  } Unfocus.
+  normalize.
+  apply SC_remove_subst.
+Qed.
